complete con hash 2

theories/coneris/examples/hash/con_hash_interface2.v
@@ -9,6 +9,10 @@ Definition coll_free (m : gmap nat nat) :=
   m !!! k1 = m !!! k2 ->
   k1 = k2.
 
+
+(* Definition NoDup_maps (m:gmap nat nat ) (m':gmap val (list nat)) := *)
+(*   NoDup ((map_to_list m).*2 ++ concat ((map_to_list m').*2)). *)
+
 Class con_hash2 `{!conerisGS Σ} (val_size:nat):= Con_Hash2
 {
   (** * Operations *)
@@ -25,56 +29,58 @@ Class con_hash2 `{!conerisGS Σ} (val_size:nat):= Con_Hash2
   hash_set_gname:Type;
   hash_tape_gname: Type;
   hash_lock_gname:Type;
+  hash_view_gname': Type;
+  hash_set_gname':Type;
   
   (** * Predicates *)
-  con_hash_inv2 (N:namespace) (f l hm: val) (P:gmap nat nat -> gmap val (list nat) -> iProp Σ) {HP: ∀ m m', Timeless (P m m')} (γ1:hash_view_gname) (γ2: hash_set_gname) (γ3:hash_tape_gname) (γ_lock:hash_lock_gname): iProp Σ;
+  con_hash_inv2 (N:namespace) (f l hm: val) (P:gmap nat nat -> gmap val (list nat) -> iProp Σ) {HP: ∀ m m', Timeless (P m m')} (γ1:hash_view_gname) (γ2: hash_set_gname) (γ3:hash_tape_gname) (γ4:hash_view_gname') (γ5:hash_set_gname') (γ_lock:hash_lock_gname): iProp Σ;
   (* concrete_seq_hash {L:seq_hashG Σ} (f:val) (m:gmap nat nat) : iProp Σ;  *)
-  hash_tape2 (α:val) (ns:list nat) (γ2: hash_set_gname) (γ3:hash_tape_gname): iProp Σ;
+  hash_tape2 (α:val) (ns:list nat) (γ2: hash_set_gname) (γ3:hash_tape_gname): iProp Σ; 
   hash_tape_auth2 (m:gmap val (list nat)) (γ2 :hash_set_gname) (γ3:hash_tape_gname): iProp Σ;
-  hash_auth2 (m:gmap nat nat) (γ:hash_view_gname) (γ2 : hash_set_gname): iProp Σ;
-  hash_frag2 (v res:nat) (γ:hash_view_gname) (γ2 : hash_set_gname): iProp Σ;
-  hash_set2 (s: nat) (γ2:hash_set_gname) : iProp Σ;
-  hash_set_frag2 (n:nat) (γ2:hash_set_gname) : iProp Σ;
+  hash_auth2 (m:gmap nat nat) (γ:hash_view_gname) (γ2 : hash_set_gname) (γ4: hash_view_gname') (γ5:hash_set_gname'): iProp Σ; 
+  hash_frag2 (v res:nat) (γ:hash_view_gname) (γ2 : hash_set_gname) (γ4:hash_view_gname'): iProp Σ;
+  hash_set2 (s: nat) (γ2:hash_set_gname) (γ5:hash_set_gname'): iProp Σ;
+  hash_set_frag2 (n:nat) (γ2: hash_set_gname)(γ5:hash_set_gname'): iProp Σ; 
   
   (** * General properties of the predicates *)
   (* #[global] concrete_seq_hash_timeless {L : seq_hashG Σ} f m :: *)
   (*   Timeless (concrete_seq_hash (L:=L) f m); *)
-  #[global] hash_tape_timeless α ns γ2 γ3::
-    Timeless (hash_tape2 α ns γ2 γ3);
+  #[global] hash_tape_timeless α ns γ2 γ3 ::
+    Timeless (hash_tape2 α ns γ2 γ3 );
   #[global] hash_tape_auth_timeless m γ2 γ3::
     Timeless (hash_tape_auth2 m γ2 γ3);
-  #[global] hash_auth_timeless m γ γ2::
-    Timeless (hash_auth2 m γ γ2);
-  #[global] hash_frag_timeless v res γ γ2::
-    Timeless (hash_frag2 v res γ γ2);
-  #[global] hash_set_timeless s γ2 ::
-    Timeless (hash_set2 s γ2); 
-  #[global] hash_set_frag_timeless s γ2 ::
-    Timeless (hash_set_frag2 s γ2); 
-  #[global] con_hash_inv_persistent N f l hm γ1 γ2 γ3 P {HP: ∀ m m', Timeless (P m m')} γ_lock ::
-    Persistent (con_hash_inv2 N f l hm P γ1 γ2 γ3 γ_lock); 
-  #[global] hash_frag_persistent v res γ γ2::
-    Persistent (hash_frag2 v res γ γ2);
-  #[global] hash_set_frag_persistent s γ2 ::
-    Persistent (hash_set_frag2 s γ2); 
-  hash_auth_exclusive m m' γ γ2:
-    hash_auth2 m γ γ2 -∗ hash_auth2 m' γ γ2 -∗ False;
-  hash_auth_frag_agree m k v γ γ2:
-    hash_auth2 m γ γ2 -∗ hash_frag2 k v γ γ2 -∗ ⌜m!!k=Some v⌝;
-  hash_auth_duplicate m k v γ γ2:
-    m!!k=Some v -> hash_auth2 m γ γ2 -∗ hash_frag2 k v γ γ2;
-  hash_auth_coll_free m γ γ2:
-    hash_auth2 m γ γ2 -∗ ⌜coll_free m⌝;
-  hash_frag_frag_agree k1 k2 v1 v2 γ γ2:
-    hash_frag2 k1 v1 γ γ2 -∗ hash_frag2 k2 v2 γ γ2-∗ ⌜k1=k2<->v1=v2⌝; 
-  hash_frag_in_hash_set γ1 γ2 v res:
-    hash_frag2 v res γ1 γ2 -∗ hash_set_frag2 res γ2 ; 
-  hash_tape_in_hash_set α ns γ γ':
-  hash_tape2 α ns γ γ' -∗ [∗ list] n ∈ ns, hash_set_frag2 n γ; 
+  #[global] hash_auth_timeless m γ γ2 γ4 γ5::
+    Timeless (hash_auth2 m γ γ2 γ4 γ5);
+  #[global] hash_frag_timeless v res γ γ2 γ4::
+    Timeless (hash_frag2 v res γ γ2 γ4);
+  #[global] hash_set_timeless s γ2 γ5::
+    Timeless (hash_set2 s γ2 γ5); 
+  #[global] hash_set_frag_timeless s γ2 γ5 ::
+    Timeless (hash_set_frag2 s γ2 γ5); 
+  #[global] con_hash_inv_persistent N f l hm γ1 γ2 γ3 P {HP: ∀ m m', Timeless (P m m')} γ4 γ5 γ_lock ::
+    Persistent (con_hash_inv2 N f l hm P γ1 γ2 γ3 γ4 γ5 γ_lock); 
+  #[global] hash_frag_persistent v res γ γ2 γ4 ::
+    Persistent (hash_frag2 v res γ γ2 γ4);
+  (* #[global] hash_set_frag_persistent s γ2 :: *)
+  (*   Persistent (hash_set_frag2 s γ2);  *)
+  hash_auth_exclusive m m' γ γ2 γ4 γ5:
+    hash_auth2 m γ γ2 γ4 γ5-∗ hash_auth2 m' γ γ2 γ4 γ5-∗ False;
+  hash_auth_frag_agree m k v γ γ2 γ4 γ5:
+    hash_auth2 m γ γ2 γ4 γ5 -∗ hash_frag2 k v γ γ2 γ4 -∗ ⌜m!!k=Some v⌝; 
+  hash_auth_duplicate m k v γ γ2 γ4 γ5:
+    m!!k=Some v -> hash_auth2 m γ γ2 γ4 γ5 -∗ hash_frag2 k v γ γ2 γ4;
+  hash_auth_coll_free m γ γ2 γ4 γ5:
+    hash_auth2 m γ γ2 γ4 γ5-∗ ⌜coll_free m⌝;
+  hash_frag_frag_agree k1 k2 v1 v2 γ γ2 γ4 :
+    hash_frag2 k1 v1 γ γ2 γ4 -∗ hash_frag2 k2 v2 γ γ2 γ4-∗ ⌜k1=k2<->v1=v2⌝; 
+  (* hash_frag_in_hash_set γ1 γ2 v res: *)
+  (*   hash_frag2 v res γ1 γ2 -∗ hash_set_frag2 res γ2 ;  *)
+  (* hash_tape_in_hash_set α ns γ γ': *)
+  (* hash_tape2 α ns γ γ' -∗ [∗ list] n ∈ ns, hash_set_frag2 n γ;  *)
   (* hash_set_frag_in_set s n γ: *)
   (* hash_set1 s γ -∗ hash_set_frag1 n γ -∗ ⌜n ∈ s⌝; *)
-  hash_auth_insert m k v γ1 γ2:
-    m!!k=None -> ([∗ map]v' ∈ m, ⌜v'≠v⌝) -∗ hash_set_frag2 v γ2 -∗ hash_auth2 m γ1 γ2 ==∗ hash_auth2 (<[k:=v]> m ) γ1 γ2; 
+  hash_auth_insert m k v γ1 γ2 γ4 γ5:
+    m!!k=None -> hash_set_frag2 v γ2 γ5 -∗ hash_auth2 m γ1 γ2 γ4 γ5 ==∗ hash_auth2 (<[k:=v]> m ) γ1 γ2 γ4 γ5  ;  
   (* hash_tape_auth_exclusive m m' γ2 γ3: *)
   (*   hash_tape_auth1 m γ2 γ3 -∗ hash_tape_auth1 m' γ2 γ3 -∗ False; *)
   (* hash_tape_auth_frag_agree m α ns γ2 γ3: *)
@@ -86,27 +92,27 @@ Class con_hash2 `{!conerisGS Σ} (val_size:nat):= Con_Hash2
   (* hash_tape_auth1 (<[α:=ns++[n]]> m) γ2 γ3 ∗ hash_tape1 α (ns ++ [n]) γ2 γ3; *) 
   (* hash_set_valid s γ: *)
   (*   hash_set1 s γ -∗ ⌜∀ n, n∈s -> (n<=val_size)%nat⌝; *)
-  hash_tape_valid α ns γ2 γ3:
-    hash_tape2 α ns γ2 γ3-∗ ⌜Forall (λ x, x<=val_size)%nat ns⌝; 
-  hash_tape_exclusive α ns ns' γ2 γ3:
-      hash_tape2 α ns γ2 γ3-∗ hash_tape2 α ns' γ2 γ3 -∗ False; 
+  hash_tape_valid α ns γ2 γ3 :
+    hash_tape2 α ns γ2 γ3 -∗ ⌜Forall (λ x, x<=val_size)%nat ns⌝; 
+  hash_tape_exclusive α ns ns' γ2 γ3 :
+      hash_tape2 α ns γ2 γ3 -∗ hash_tape2 α ns' γ2 γ3  -∗ False; 
 
   
-  hash_tape_presample m γ γ_set α ns n (ε εO:nonnegreal) E:
-    (INR n + εO * (val_size + 1 - INR n) <= ε * (val_size + 1))%R ->
-    hash_tape_auth2 m γ_set γ -∗ hash_tape2 α ns γ_set γ -∗ ↯ ε -∗
-    hash_set2 n γ_set -∗
+  hash_tape_presample m γ γ_set γ_set' α ns s (ε εO:nonnegreal) E:
+    (INR s + εO * (val_size + 1 - INR s) <= ε * (val_size + 1))%R ->
+    hash_tape_auth2 m γ_set γ -∗ hash_tape2 α ns γ_set γ-∗ ↯ ε -∗
+    hash_set2 s γ_set γ_set'-∗
     state_update E E (∃ (n:fin(S val_size)), 
-          (  hash_set2 (n+1)%nat γ_set ∗ ↯ εO
+          (  hash_set2 (s+1)%nat γ_set γ_set' ∗ ↯ εO
           )∗
           hash_tape_auth2 (<[α:=ns++[fin_to_nat n]]>m) γ_set γ ∗
-          hash_tape2 α (ns++[fin_to_nat n]) γ_set γ
-      ); 
+          hash_tape2 α (ns++[fin_to_nat n]) γ_set γ ∗ hash_set_frag2 (fin_to_nat n) γ_set γ_set'
+      );
 
-  con_hash_presample2  N f l hm P {HP: ∀ m m', Timeless (P m m')} γ_hv γ_set γ_tape γ_lock Q
+  con_hash_presample2  N f l hm P {HP: ∀ m m', Timeless (P m m')} γ_hv γ_set γ_tape γ_hv' γ_set' γ_lock Q
     E  :
     ↑N ⊆ E ->
-    con_hash_inv2 N f l hm P γ_hv γ_set γ_tape γ_lock -∗
+    con_hash_inv2 N f l hm P γ_hv γ_set γ_tape γ_hv' γ_set' γ_lock -∗
     (∀ m m', P m m'  -∗
              hash_tape_auth2 m' γ_set γ_tape -∗
              state_update (E∖↑N) (E∖↑N)
@@ -119,26 +125,27 @@ Class con_hash2 `{!conerisGS Σ} (val_size:nat):= Con_Hash2
   con_hash_init2 N P {HP: ∀ m m', Timeless (P m m')}:
     {{{ P ∅ ∅ }}}
       init_hash2 #()
-      {{{ (f:val), RET f; ∃ l hm γ1 γ2 γ3 γ_lock, con_hash_inv2 N f l hm P γ1 γ2 γ3 γ_lock ∗
-                                                  hash_set2 0%nat γ2
+      {{{ (f:val), RET f; ∃ l hm γ1 γ2 γ3 γ4 γ5 γ_lock, con_hash_inv2 N f l hm P γ1 γ2 γ3 γ4 γ5 γ_lock ∗
+                                                  hash_set2 0%nat γ2 γ5
       }}}; 
 
-  con_hash_alloc_tape2 N f l hm P {HP: ∀ m m', Timeless (P m m')} γ1 γ2 γ3 γ_lock Q:
-  {{{ con_hash_inv2 N f l hm P γ1 γ2 γ3 γ_lock ∗
+  con_hash_alloc_tape2 N f l hm P {HP: ∀ m m', Timeless (P m m')} γ1 γ2 γ3 γ4 γ5 γ_lock Q:
+  {{{ con_hash_inv2 N f l hm P γ1 γ2 γ3 γ4 γ5 γ_lock ∗
       (∀ m m' α, P m m' -∗ ⌜α∉dom m'⌝ -∗ |={⊤∖↑N}=> P m (<[α:=[]]>m') ∗ Q α)
   }}}
       allocate_tape2 #()
       {{{ (α: val), RET α; hash_tape2 α [] γ2 γ3 ∗ Q α }}};  
 
-  con_hash_spec2 N f l hm P {HP: ∀ m m', Timeless (P m m')} γ1 γ2 γ3 γ_lock Q1 Q2 α ns (v:nat):
-  {{{ con_hash_inv2 N f l hm P γ1 γ2 γ3 γ_lock ∗ hash_tape2 α (ns) γ2 γ3∗
+  con_hash_spec2 N f l hm P {HP: ∀ m m', Timeless (P m m')} γ1 γ2 γ3 γ4 γ5 γ_lock Q1 Q2 α ns (v:nat):
+  {{{ con_hash_inv2 N f l hm P γ1 γ2 γ3 γ4 γ5 γ_lock ∗ hash_tape2 α (ns) γ2 γ3∗
       ( ∀ m m', P m m' -∗
-                hash_auth2 m γ1 γ2 -∗
+                hash_auth2 m γ1 γ2 γ4 γ5-∗
                 ⌜m'!!α=Some ns⌝ -∗
-                ([∗ map]v' ∈ m, ⌜Forall (λ n, n≠v') ns⌝) -∗ |={⊤∖↑N}=>
+                |={⊤∖↑N}=>
              match m!!v with
-             | Some res => P m m' ∗ hash_auth2 m γ1 γ2 ∗ Q1 res
-             | None => ∃ n ns', ⌜n::ns'=ns⌝ ∗ P (<[v:=n]> m) (<[α:=ns']> m')∗ hash_auth2 (<[v:=n]> m) γ1 γ2  ∗ Q2
+             | Some res => P m m' ∗ hash_auth2 m γ1 γ2 γ4 γ5 ∗ Q1 res
+             | None => ∃ n ns', ⌜n::ns'=ns⌝ ∗ P (<[v:=n]> m) (<[α:=ns']> m')∗ hash_auth2 (<[v:=n]> m) γ1 γ2 γ4 γ5 ∗
+                                 Q2
              end                                        
       )
   }}}
@@ -152,72 +159,69 @@ Class con_hash2 `{!conerisGS Σ} (val_size:nat):= Con_Hash2
 
 Section test.
   Context `{conerisGS Σ, !con_hash2 val_size}.
+  Definition hash_tape2' α ns γ2 γ3 γ5:= (hash_tape2 α ns γ2 γ3 ∗ [∗ list] n∈ns, hash_set_frag2 n γ2 γ5)%I.
+                                                    
 
-  Lemma con_hash_presample_test N f l hm γ1 γ2 γ3 γlock  E (ε εI εO:nonnegreal) ns α n :
+  Lemma con_hash_presample_test N f l hm γ1 γ2 γ3 γ4 γ5 γlock  E (ε εI εO:nonnegreal) ns α s :
     ↑N⊆E ->
-    (INR n + εO * (val_size + 1 - INR n) <= ε * (val_size + 1))%R ->
-    con_hash_inv2 N f l hm (λ _ _, True) γ1 γ2 γ3 γlock -∗
-    hash_tape2 α ns γ2 γ3 -∗
+    (INR s+ εO * (val_size + 1 - INR s) <= ε * (val_size + 1))%R ->
+    con_hash_inv2 N f l hm (λ _ _, True) γ1 γ2 γ3 γ4 γ5 γlock -∗
+    hash_tape2' α ns γ2 γ3 γ5-∗
     ↯ ε -∗
-    hash_set2 n γ2 -∗
+    hash_set2 s γ2 γ5-∗
     state_update E E (∃ (n:fin (S val_size)),
-          hash_tape2 α (ns++[fin_to_nat n]) γ2 γ3 ∗
-          ( hash_set2 (n+1)%nat γ2 ∗ ↯ εO
+          hash_tape2' α (ns++[fin_to_nat n]) γ2 γ3 γ5 ∗
+          ( hash_set2 (s+1)%nat γ2 γ5∗ ↯ εO
           )
       ).
   Proof.
-    iIntros (Hsubset Hineq) "#Hinv Ht Herr Hs".
-    iMod (con_hash_presample2 _ _ _ _ _ _ _ _ _
+    iIntros (Hsubset Hineq) "#Hinv [Ht Hfrag] Herr Hs".
+    iMod (con_hash_presample2 _ _ _ _ _ _ _ _ _ _ _
             (λ m m' m'', (∃ n : fin (S val_size), hash_tape2 α (ns ++ [fin_to_nat n]) γ2 γ3 ∗
-                                                  ( hash_set2 (n +1)%nat γ2 ∗ ↯ εO)))%I with "[//][-]") as "Hcont"; first done.
+                                                  ( hash_set2 (s +1)%nat γ2 γ5 ∗ ↯ εO) ∗ hash_set_frag2 (fin_to_nat n) _ _))%I with "[//][-Hfrag]") as "Hcont"; first done.
     - iIntros (_ ?) "_ Hauth".
-      iMod (hash_tape_presample with "[$][$][$][$]") as "(%&?&$&$)"; first done.
-      by iFrame.
-    - by iDestruct "Hcont" as "(%&%&%&%&$&$&$)". 
+      by iMod (hash_tape_presample with "[$][$][$][$]") as "(%&[$$]&$&$&?)". 
+    - iFrame. iDestruct "Hcont" as "(%&%&%&%&$&$&$)". by iModIntro.
   Qed.
   
     
-  Lemma con_hash_spec_test2 N f l hm γ1 γ2 γ3 γlock α n ns (v:nat):
-    {{{ con_hash_inv2 N f l hm (λ _ _, True) γ1 γ2 γ3 γlock ∗ hash_tape2 α (n::ns) γ2 γ3 }}}
+  Lemma con_hash_spec_test2 N f l hm γ1 γ2 γ3 γ4 γ5 γlock α n ns (v:nat):
+    {{{ con_hash_inv2 N f l hm (λ _ _, True) γ1 γ2 γ3 γ4 γ5 γlock ∗ hash_tape2' α (n::ns) γ2 γ3 γ5 }}}
       f #v α
-      {{{ (res:nat), RET (#res);  hash_frag2 v res γ1 γ2 ∗
-                                (hash_tape2 α ns γ2 γ3 ∗ ⌜res=n⌝ ∨
-                                 hash_tape2 α (n::ns) γ2 γ3
+      {{{ (res:nat), RET (#res);  hash_frag2 v res γ1 γ2 γ4 ∗
+                                (hash_tape2' α ns γ2 γ3 γ5 ∗ ⌜res=n⌝ ∨
+                                 hash_tape2' α (n::ns) γ2 γ3 γ5
                                 )
       }}}.
   Proof.
-    iIntros (Φ) "[#Hinv Ht] HΦ".
-    iDestruct (hash_tape_in_hash_set with "[$]") as "#Hfrag".
-    iApply (con_hash_spec2 _ _ _ _ _ _ _ _ _ (λ res, hash_frag2 v res γ1 γ2) (hash_frag2 v n γ1 γ2) with "[$Hinv $Ht]").
-    - iIntros (??) "_ Hauth % %H'".
+    iIntros (Φ) "[#Hinv [Ht Hlis]] HΦ".
+    iApply (con_hash_spec2 _ _ _ _ _ _ _ _ _ _ _ (λ res, hash_frag2 v res γ1 γ2 γ4 ∗ [∗ list] n0 ∈ (n :: ns), hash_set_frag2 n0 γ2 γ5)%I (hash_frag2 v n γ1 γ2 γ4 ∗ [∗ list] n0 ∈ (ns), hash_set_frag2 n0 γ2 γ5) with "[$Hinv $Ht Hlis]").
+    - iIntros (??) "_ Hauth %".
       case_match.
-      + by iDestruct (hash_auth_duplicate with "[$]") as "#$"; first done.
-      + iMod (hash_auth_insert with "[][][$]") as "H"; first done; last first.
-        * iDestruct (hash_auth_duplicate with "[$]") as "#$"; first by rewrite lookup_insert.
-          iFrame. iModIntro. by iExists _.
-        * rewrite big_sepL_cons. iDestruct "Hfrag" as "[$ ?]".
-        * iPureIntro. intros ?? H2.
-          apply H' in H2. rewrite Forall_cons in H2.
-          simpl in *. naive_solver.
-    - iNext. iIntros (res) "[[??]|(%&%&%&?&%&H)]".
-      + iApply "HΦ". iFrame.
+      + iDestruct (hash_auth_duplicate with "[$]") as "#$"; first done. by iFrame.
+      + iDestruct "Hlis" as "[H1 Hlis]".
+        iMod (hash_auth_insert with "[$][$]") as "H"; first done.
+        iDestruct (hash_auth_duplicate with "[$]") as "#$"; first by rewrite lookup_insert.
+        iFrame. iModIntro. iExists _. done.
+    - iNext. iIntros (res) "[(?&?&?)|(%&%&%&?&%&H&?)]".
+      + iApply "HΦ". iFrame. iRight. iFrame.
       + iApply "HΦ". simplify_eq. iFrame "H". iLeft. by iFrame.
   Qed.
 
-  Lemma con_hash_spec_hashed_before2 N f l hm γ1 γ2 γ3 γlock α ns res (v:nat):
-    {{{ con_hash_inv2 N f l hm (λ _ _, True) γ1 γ2 γ3 γlock ∗ hash_tape2 α ns γ2 γ3 ∗ hash_frag2 v res γ1 γ2 }}}
+  Lemma con_hash_spec_hashed_before2 N f l hm γ1 γ2 γ3 γ4 γ5 γlock α ns res (v:nat):
+    {{{ con_hash_inv2 N f l hm (λ _ _, True) γ1 γ2 γ3 γ4 γ5 γlock ∗ hash_tape2' α ns γ2 γ3 γ5 ∗ hash_frag2 v res γ1 γ2 γ4}}}
       f #v α
-      {{{ RET (#res);  hash_frag2 v res γ1 γ2 ∗
-                       (hash_tape2 α ns γ2 γ3 )
+      {{{ RET (#res);  hash_frag2 v res γ1 γ2 γ4 ∗
+                       (hash_tape2' α ns γ2 γ3 γ5)
       }}}.
   Proof. 
-    iIntros (Φ) "(#Hinv & Ht & #Hf) HΦ".
-    iDestruct (hash_tape_in_hash_set with "[$]") as "#Hfrag".
-    iApply (con_hash_spec2 _ _ _ _ _ _ _ _ _ (λ res' , ⌜res=res'⌝ ∗ hash_frag2 v res γ1 γ2)%I (False) with "[$Hinv $Ht]").
+    iIntros (Φ) "(#Hinv & [Ht ?] & #Hf) HΦ".
+    iApply (con_hash_spec2 _ _ _ _ _ _ _ _ _ _ _(λ res' , ⌜res=res'⌝ ∗ hash_frag2 v res γ1 γ2 γ4  )%I (False) with "[$Hinv $Ht]").
     - iIntros (??) "_ Hauth %".
       case_match.
       + iDestruct (hash_auth_frag_agree with "[$][$]") as "%".
-        simplify_eq. iDestruct (hash_auth_duplicate with "[$]") as "#$"; first done. by iFrame.
+        simplify_eq. iDestruct (hash_auth_duplicate with "[$]") as "#$"; first done.
+        iFrame. by done. 
       + iDestruct (hash_auth_frag_agree with "[$][$]") as "%".
         simplify_eq.
     - iNext. iIntros (res') "[[?[->?]]|(%&%&%&?&?&%)]".
