theories/coneris/examples/hash/con_hash_impl2.v
@@ -1,0 +1,260 @@
+From stdpp Require Import namespaces finite fin_sets.
+From iris.proofmode Require Import proofmode.
+From iris.algebra Require Import excl_auth gmap.
+From clutch.prelude Require Import stdpp_ext.
+From clutch.coneris Require Import coneris coll_free_hash_view_interface con_hash_interface1 con_hash_interface2.
+
+Set Default Proof Using "Type*".
+
+Section con_hash_impl2.
+  
+  Variable val_size:nat.
+  Context `{Hc: conerisGS Σ, 
+              h : @hash_view Σ Hc, Hhv: hvG Σ,
+                Hs: !ghost_mapG Σ nat (),
+               hash1: !con_hash1 val_size
+    }.
+
+  (** * Code *)
+
+  Definition init_hash:=init_hash1.
+  Definition compute_hash:=compute_hash1.
+  Definition allocate_tape:=allocate_tape1.
+
+  
+  Definition hash_set_frag v γ_set γ_set' := (hash_set_frag1 v γ_set∗ (v ↪[γ_set'] ()))%I.
+  Definition hash_set n γ γ':=
+    (∃ s, ⌜size s = n⌝ ∗ hash_set1 s γ ∗ ghost_map_auth γ' 1 (gset_to_gmap () s))%I.
+  
+  Definition hash_auth m γ1 γ2 γ4 γ5:=
+    (hv_auth (L:=Hhv) m γ4 ∗
+     hash_auth1 m γ1 γ2 ∗
+     ([∗ map] v∈m, hash_set_frag v γ2 γ5) 
+    )%I.
+  Definition hash_tape α ns γ2 γ_tape :=
+    (hash_tape1 α ns γ2 γ_tape (* ∗ [∗ list] n∈ns, hash_set_frag n γ5 *))%I.
+  Definition hash_tape_auth m γ2 γ3 :=
+    (hash_tape_auth1 m γ2 γ3
+    )%I.
+
+  Definition hash_frag k v γ1 γ2 γ4:=
+    (hv_frag (L:=Hhv) k v γ4 ∗
+     hash_frag1 k v γ1 γ2)%I.
+
+  Definition con_hash_inv N f l hm (P:gmap nat nat -> gmap val (list nat) -> iProp Σ) {HP: ∀ m m', Timeless (P m m')} γ1 γ2 γ_tape γ4 γ5 γ_lock:=
+    con_hash_inv1 N f l hm (λ m m', hv_auth (L:=Hhv) m γ4 ∗ ([∗ map] v∈m, (v ↪[γ5] ())) ∗ P m m')%I γ1 γ2  γ_tape γ_lock.
+
+  Lemma hash_tape_presample m γ γ_set γ_set' α ns s (ε εO:nonnegreal) E:
+    (INR s + εO * (val_size + 1 - INR s) <= ε * (val_size + 1))%R ->
+    hash_tape_auth m γ_set γ -∗ hash_tape α ns γ_set γ-∗ ↯ ε -∗
+    hash_set s γ_set γ_set'-∗
+    state_update E E (∃ (n:fin(S val_size)), 
+          (  hash_set (s+1)%nat γ_set γ_set' ∗ ↯ εO
+          )∗
+          hash_tape_auth (<[α:=ns++[fin_to_nat n]]>m) γ_set γ ∗
+          hash_tape α (ns++[fin_to_nat n]) γ_set γ ∗ hash_set_frag (fin_to_nat n) γ_set γ_set'
+      ).
+  Proof.
+    rewrite /hash_tape_auth/hash_tape/hash_set/hash_set_frag.
+    iIntros (Hineq) "Htauth Ht Herr (%s' & <- & Hset & Hset')".
+    iMod (con_hash_interface1.hash_tape_presample _ _ _ _ _ _ _ 1%NNR with "[$][$][$][$]") as "Hcont".
+    { simpl. erewrite Rmult_1_l. done. }
+    iDestruct ("Hcont" ) as "(%&[(%&?&?)|(%&?&?)]&$&$)".
+    { by iDestruct (ec_contradict with "[$]") as "%". }
+    iMod (ghost_map_insert with "[$]") as "[Hset' Hs']".
+    { apply not_elem_of_dom_1. by rewrite dom_gset_to_gmap. }
+    rewrite <-gset_to_gmap_union_singleton. 
+    iModIntro. iFrame.
+    repeat iSplit; try done.
+    - iPureIntro. rewrite size_union; last set_solver. rewrite size_singleton. lia.
+    - by rewrite union_comm_L.
+    - iApply (hash_set_duplicate); last done. set_solver.
+  Qed.
+    
+  Lemma con_hash_presample N f l hm P {HP: ∀ m m', Timeless (P m m')} γ_hv γ_set γ_tape γ_hv' γ_set' γ_lock Q
+    E  :
+    ↑N ⊆ E ->
+    con_hash_inv N f l hm P γ_hv γ_set γ_tape γ_hv' γ_set' γ_lock -∗
+    (∀ m m', P m m'  -∗
+             hash_tape_auth m' γ_set γ_tape -∗
+             state_update (E∖↑N) (E∖↑N)
+             (∃ m'', P m m'' ∗ hash_tape_auth m'' γ_set γ_tape ∗ Q m m' m'')
+    ) -∗
+    state_update E E (
+        ∃ m m' m'', Q m m' m''
+      ).
+  Proof.
+    iIntros (Hsubset) "#Hinv Hvs".
+    iMod (con_hash_presample1 with "[//][-]"); first done; last done.
+    rewrite /hash_tape_auth.
+    iIntros (??) "($&$&?)?".
+    by iMod ("Hvs" with "[$][$]") as "(%&$&$)".
+  Qed.
+
+  Lemma con_hash_init N P {HP: ∀ m m', Timeless (P m m')}:
+    {{{ P ∅ ∅ }}}
+      init_hash #()
+      {{{ (f:val), RET f; ∃ l hm γ1 γ2 γ3 γ4 γ5 γ_lock, con_hash_inv N f l hm P γ1 γ2 γ3 γ4 γ5 γ_lock ∗
+                                                  hash_set 0%nat γ2 γ5
+      }}}.
+  Proof.
+    iIntros (Φ) "HP HΦ".
+    rewrite /init_hash.
+    iApply fupd_pgl_wp.
+    iMod (hv_auth_init) as "(%γ1'&H)".
+    iMod (ghost_map_alloc_empty) as "(%γ2' &H')".
+    iModIntro.
+    wp_apply (con_hash_init1 _  with "[HP H]"); last first.
+    - iIntros (f)"(%l &%hm&%γ1&%γ2&%γ3&%γ_lock&#H1&H2)".
+      iApply "HΦ". rewrite /con_hash_inv/hash_set.
+      by iFrame "H1 H2 H'".
+    - by iFrame.
+  Qed.
+
+  Lemma con_hash_alloc_tape N f l hm P {HP: ∀ m m', Timeless (P m m')} γ1 γ2 γ3 γ4 γ5 γ_lock Q:
+  {{{ con_hash_inv N f l hm P γ1 γ2 γ3 γ4 γ5 γ_lock ∗
+      (∀ m m' α, P m m' -∗ ⌜α∉dom m'⌝ -∗ |={⊤∖↑N}=> P m (<[α:=[]]>m') ∗ Q α)
+  }}}
+      allocate_tape #()
+      {{{ (α: val), RET α; hash_tape α [] γ2 γ3 ∗ Q α }}}.
+  Proof.
+    iIntros (Φ) "[#Hinv Hvs] HΦ".
+    rewrite /allocate_tape.
+    wp_apply (con_hash_alloc_tape1 with "[Hvs $Hinv]").
+    - iIntros (???) "(?&?&?)%".
+      iMod ("Hvs" with "[$][//]") as "[$ H]".
+      iFrame.
+      iApply "H".
+    - rewrite /hash_tape.
+      iIntros (?) "[??]".
+      iApply "HΦ". iFrame.
+  Qed.
+
+  Lemma con_hash_spec N f l hm P {HP: ∀ m m', Timeless (P m m')} γ1 γ2 γ3 γ4 γ5 γ_lock Q1 Q2 α ns (v:nat):
+  {{{ con_hash_inv N f l hm P γ1 γ2 γ3 γ4 γ5 γ_lock ∗ hash_tape α (ns) γ2 γ3∗
+      ( ∀ m m', P m m' -∗
+                hash_auth m γ1 γ2 γ4 γ5-∗
+                ⌜m'!!α=Some ns⌝ -∗
+                |={⊤∖↑N}=>
+             match m!!v with
+             | Some res => P m m' ∗ hash_auth m γ1 γ2 γ4 γ5 ∗ Q1 res
+             | None => ∃ n ns', ⌜n::ns'=ns⌝ ∗ P (<[v:=n]> m) (<[α:=ns']> m')∗ hash_auth (<[v:=n]> m) γ1 γ2 γ4 γ5 ∗
+                                 Q2
+             end                                        
+      )
+  }}}
+      f #v α
+      {{{ (res:nat), RET (#res);  (hash_tape α (ns) γ2 γ3 ∗ Q1 res ∨
+                                 ∃ n ns', ⌜n::ns'=ns⌝ ∗ hash_tape α ns' γ2 γ3 ∗ ⌜res=n⌝ ∗ Q2 
+                                )
+      }}}.
+  Proof.
+    iIntros (Φ) "(#Hinv & Ht & Hvs) HΦ".
+    rewrite /hash_tape/hash_set_frag.
+    iApply (con_hash_spec1 _ _ _ _ _ _ _ _ _ Q1 Q2 with "[$Hinv $Ht Hvs]").
+    - iIntros (??) "(Hhv & Hfrag & HP) Hauth1 %H".
+      rewrite /hash_auth.
+      rewrite /hash_set_frag.
+      iMod ("Hvs" with "[$][Hauth1 $Hhv Hfrag][//]") as "Hcont".
+      { rewrite big_sepM_sep. iFrame "Hfrag". iSplit; first done.
+        rewrite big_sepM_forall. iIntros.
+        iDestruct (con_hash_interface1.hash_auth_duplicate with "[$]") as "#?"; first done.
+        by iApply hash_frag_in_hash_set.
+      }
+      case_match.
+      + iDestruct "Hcont" as "($&($&?&H)&$)".
+        iFrame.
+        rewrite big_sepM_sep.
+        by iDestruct "H" as "[??]".
+      + iDestruct "Hcont" as "(%&%&<-&$&($&$&H)&$)".
+        rewrite big_sepM_sep.
+        iDestruct "H" as "[??]". by iFrame.
+    - iNext. iIntros (?) "[?|(%&%&<-&?&?)]"; iApply "HΦ".
+      + iLeft. by iFrame.
+      + iRight. by iFrame.
+  Qed.
+      
+  
+  Program Definition con_hash_impl2 : con_hash2 val_size :=
+    {| init_hash2:=init_hash;
+      allocate_tape2:=allocate_tape;
+      compute_hash2:=compute_hash;
+      
+      con_hash_inv2 := con_hash_inv; 
+      hash_tape2:=hash_tape;
+      hash_frag2:=hash_frag;
+      hash_auth2:=hash_auth;
+      hash_tape_auth2 := hash_tape_auth;
+      hash_set2:=hash_set; 
+      hash_set_frag2:=hash_set_frag; 
+      con_hash_interface2.hash_tape_presample := hash_tape_presample; 
+      con_hash_presample2 := con_hash_presample; 
+      con_hash_init2 := con_hash_init; 
+      con_hash_alloc_tape2 := con_hash_alloc_tape; 
+      con_hash_spec2:=con_hash_spec
+    |}
+  .
+  Next Obligation.
+    iIntros (??????) "[??][??]".
+    iApply (hv_auth_exclusive with "[$][$]").
+  Qed.
+  Next Obligation.
+    iIntros (???????)"[??][??]".
+    iApply (hv_auth_frag_agree with "[$]").
+  Qed.
+  Next Obligation.
+    iIntros (????????) "[?[??]]".
+    iDestruct (hv_auth_duplicate_frag with "[$]") as "[? $]"; first done.
+    by iApply (con_hash_interface1.hash_auth_duplicate).
+  Qed.
+  Next Obligation.
+    iIntros (?????) "[??]".
+    by iApply hv_auth_coll_free.
+  Qed.
+  Next Obligation.
+    rewrite /hash_frag.
+    iIntros (???????) "[??][??]".
+    iDestruct (hv_frag_frag_agree with "[$][$]") as "%". iPureIntro. naive_solver.
+  Qed.
+  Next Obligation.
+    iIntros (????????) "[H1 H2][H3[H4 H5]]".
+    rewrite /hash_set_frag.
+    rewrite big_sepM_sep.
+    iDestruct "H5" as "[#H5 H6]".
+    rewrite /hash_auth.
+    iMod (con_hash_interface1.hash_auth_insert with "[$][$]") as "K"; first done.
+    iDestruct (con_hash_interface1.hash_auth_duplicate with "[$]") as "#?"; first apply lookup_insert.
+    iAssert (⌜v∉(map_to_list m).*2⌝)%I as "%H0".
+    { iIntros (H').
+      apply elem_of_list_fmap_2 in H'.
+      destruct H' as ([??]&?&H1). simplify_eq.
+      rewrite elem_of_map_to_list in H1.
+      iDestruct (big_sepM_lookup with "[$]") as "H4"; first done.
+      simpl.
+      iCombine "H2 H4" gives "%H0".
+      cbv in H0. naive_solver.
+    } 
+    iMod (hv_auth_insert with "[$]") as "[$?]"; first done.
+    { rewrite Forall_forall.
+      intros x Hx.
+      intros ->.
+      by apply H0. }
+    rewrite big_sepM_insert; last done.
+    iFrame.
+    iDestruct (hash_frag_in_hash_set with "[$]") as "$".
+    rewrite /hash_set_frag.
+    iModIntro. rewrite big_sepM_sep.
+    by iFrame.
+  Qed.
+  
+  Next Obligation.
+    iIntros (????) "?".
+    by iApply con_hash_interface1.hash_tape_valid.
+  Qed.
+  Next Obligation.
+    iIntros (?????) "??".
+    iApply (con_hash_interface1.hash_tape_exclusive with "[$][$]").
+  Qed.
+
+  
+End con_hash_impl2.
